Switch to a mutually recursive typing judgement
Also restore divided induction rules for ease of use

Typing.thy
@@ -2,40 +2,77 @@ theory Typing
   imports Syntax Defs
 begin
 
-inductive Ty :: "\<Gamma> \<Rightarrow> \<tau> \<Rightarrow> \<kappa> \<Rightarrow> bool" ("_ \<turnstile>\<^sub>t\<^sub>y _ : _") where
-  Ty_Unit: "\<Gamma> \<turnstile>\<^sub>t\<^sub>y TyUnit : \<star>"
+no_notation Set.member  ("(_/ : _)" [51, 51] 50)
 
-| Ty_Var: "BTyVar a k \<in> \<Gamma> \<Longrightarrow> \<Gamma> \<turnstile>\<^sub>t\<^sub>y TyVar a : k"
+inductive Ctx :: "\<Gamma> \<Rightarrow> bool" ("\<turnstile> _")
+  and Ty :: "\<Gamma> \<Rightarrow> \<tau> \<Rightarrow> \<kappa> \<Rightarrow> bool" ("_ \<turnstile>\<^sub>t\<^sub>y _ : _")
+  and Tm :: "\<Gamma> \<Rightarrow> term \<Rightarrow> \<tau> \<Rightarrow> bool" ("_ \<turnstile> _ : _" 50) where
 
-| Ty_Arrow: "\<lbrakk> \<Gamma> \<turnstile>\<^sub>t\<^sub>y \<tau>1 : \<star> ; \<Gamma> \<turnstile>\<^sub>t\<^sub>y \<tau>2 : \<star> \<rbrakk> \<Longrightarrow> \<Gamma> \<turnstile>\<^sub>t\<^sub>y (\<tau>1 \<rightarrow> \<tau>2) : \<star>"
+  Ctx_Empty: "\<turnstile> []"
+
+| Ctx_TyVar: "\<lbrakk> \<turnstile> \<Gamma> ; atom a \<sharp> \<Gamma> \<rbrakk> \<Longrightarrow> \<turnstile> BTyVar a k # \<Gamma>"
+
+| Ctx_Var: "\<lbrakk> \<Gamma> \<turnstile>\<^sub>t\<^sub>y \<tau> : \<star> ; atom x \<sharp> \<Gamma> \<rbrakk> \<Longrightarrow> \<turnstile> BVar x \<tau> # \<Gamma>"
+
+(* ------------------------------ *)
+
+| Ty_Var: "\<lbrakk> \<turnstile> \<Gamma> ; BTyVar a k \<in> \<Gamma> \<rbrakk> \<Longrightarrow> \<Gamma> \<turnstile>\<^sub>t\<^sub>y TyVar a : k"
 
 | Ty_App: "\<lbrakk> \<Gamma> \<turnstile>\<^sub>t\<^sub>y \<tau>1 : KArrow \<kappa>1 \<kappa>2 ; \<Gamma> \<turnstile>\<^sub>t\<^sub>y \<tau>2 : \<kappa>1 \<rbrakk> \<Longrightarrow> \<Gamma> \<turnstile>\<^sub>t\<^sub>y TyConApp \<tau>1 \<tau>2 : \<kappa>2"
 
-| Ty_Forall: "\<lbrakk> BTyVar a k # \<Gamma> \<turnstile>\<^sub>t\<^sub>y \<sigma> : \<star> ; atom a \<sharp> \<Gamma> \<rbrakk> \<Longrightarrow> \<Gamma> \<turnstile>\<^sub>t\<^sub>y (\<forall>a : k. \<sigma>) : \<star>"
-equivariance Ty
-nominal_inductive Ty avoids
-  Ty_Forall: a
-  by (auto simp: fresh_star_def)
+| Ty_Unit: "\<Gamma> \<turnstile>\<^sub>t\<^sub>y TyUnit : \<star>" (* to be replaced with ADTs *)
 
-inductive T :: "\<Gamma> \<Rightarrow> term \<Rightarrow> \<tau> \<Rightarrow> bool" ("_ \<turnstile> _ : _" 50) where
-  T_UnitI: "(\<Gamma> \<turnstile> Unit : TyUnit)"
+| Ty_FunArrow: "\<lbrakk> \<Gamma> \<turnstile>\<^sub>t\<^sub>y \<tau>1 : \<star> ; \<Gamma> \<turnstile>\<^sub>t\<^sub>y \<tau>2 : \<star> \<rbrakk> \<Longrightarrow> \<Gamma> \<turnstile>\<^sub>t\<^sub>y (\<tau>1 \<rightarrow> \<tau>2) : \<star>" (* also to be a type constant *)
 
-| T_VarI: "\<lbrakk> BVar x \<tau> \<in> \<Gamma> \<rbrakk> \<Longrightarrow> \<Gamma> \<turnstile> (Var x) : \<tau>"
+| Ty_Forall: "\<lbrakk> BTyVar a k # \<Gamma> \<turnstile>\<^sub>t\<^sub>y \<sigma> : \<star> \<rbrakk> \<Longrightarrow> \<Gamma> \<turnstile>\<^sub>t\<^sub>y (\<forall>a : k. \<sigma>) : \<star>"
 
-| T_AbsI: "\<lbrakk> atom x \<sharp> \<Gamma> ; \<Gamma> \<turnstile>\<^sub>t\<^sub>y \<tau>1 : \<star> ; BVar x \<tau>1 # \<Gamma> \<turnstile> e : \<tau>2 \<rbrakk> \<Longrightarrow> \<Gamma> \<turnstile> (\<lambda> x : \<tau>1 . e) : (\<tau>1 \<rightarrow> \<tau>2)"
+(* ------------------------------ *)
 
-| T_AppI: "\<lbrakk> \<Gamma> \<turnstile> e1 : (\<tau>1 \<rightarrow> \<tau>2) ; \<Gamma> \<turnstile> e2 : \<tau>1 \<rbrakk> \<Longrightarrow> \<Gamma> \<turnstile> App e1 e2 : \<tau>2"
+| Tm_Var: "\<lbrakk> \<turnstile> \<Gamma> ; BVar x \<tau> \<in> \<Gamma> \<rbrakk> \<Longrightarrow> \<Gamma> \<turnstile> (Var x) : \<tau>"
 
-| T_LetI: "\<lbrakk> atom x \<sharp> (\<Gamma>, e1) ; BVar x \<tau>1 # \<Gamma> \<turnstile> e2 : \<tau>2 ; \<Gamma> \<turnstile> e1 : \<tau>1 \<rbrakk> \<Longrightarrow> \<Gamma> \<turnstile> Let x \<tau>1 e1 e2 : \<tau>2"
+| Tm_Abs: "BVar x \<tau>1 # \<Gamma> \<turnstile> e : \<tau>2 \<Longrightarrow> \<Gamma> \<turnstile> (\<lambda> x : \<tau>1 . e) : (\<tau>1 \<rightarrow> \<tau>2)"
 
-| T_AppTI: "\<lbrakk> \<Gamma> \<turnstile> e : (\<forall>a : k . \<sigma>) ; \<Gamma> \<turnstile>\<^sub>t\<^sub>y \<tau> : k \<rbrakk> \<Longrightarrow> \<Gamma> \<turnstile> TyApp e \<tau> : subst_type \<tau> a \<sigma>"
+| Tm_App: "\<lbrakk> \<Gamma> \<turnstile> e1 : (\<tau>1 \<rightarrow> \<tau>2) ; \<Gamma> \<turnstile> e2 : \<tau>1 \<rbrakk> \<Longrightarrow> \<Gamma> \<turnstile> App e1 e2 : \<tau>2"
 
-| T_AbsTI: "\<lbrakk> BTyVar a k # \<Gamma> \<turnstile> e : \<sigma> ; atom a \<sharp> \<Gamma> \<rbrakk> \<Longrightarrow> \<Gamma> \<turnstile> (\<Lambda> a : k . e) : (\<forall> a : k . \<sigma>)"
-equivariance T
-nominal_inductive T avoids
-  T_AbsI: x
-  | T_LetI: x
-  | T_AbsTI: a
-  by (auto simp: fresh_star_def fresh_Unit fresh_Pair)
+| Tm_TAbs: "BTyVar a k # \<Gamma> \<turnstile> e : \<sigma> \<Longrightarrow> \<Gamma> \<turnstile> (\<Lambda> a : k . e) : (\<forall> a : k . \<sigma>)"
+
+| Tm_TApp: "\<lbrakk> \<Gamma> \<turnstile> e : \<forall> a:k. \<sigma> ; \<Gamma> \<turnstile>\<^sub>t\<^sub>y \<tau> : k \<rbrakk> \<Longrightarrow> \<Gamma> \<turnstile> TyApp e \<tau> : \<sigma>[\<tau>/a]"
+
+| Tm_Unit: "\<Gamma> \<turnstile> Unit : TyUnit" (* to be replaced with ADTs *)
+
+| Tm_Let: "\<lbrakk> \<Gamma> \<turnstile> e1 : \<tau>1 ; BVar x \<tau>1 # \<Gamma> \<turnstile> e2 : \<tau>2 \<rbrakk> \<Longrightarrow> \<Gamma> \<turnstile> Let x \<tau>1 e1 e2 : \<tau>2"
+
+equivariance Ctx
+nominal_inductive Ctx .
+
+lemma Ctx_induct[consumes 1, case_names Empty TyVar Var]:
+  assumes "\<turnstile> \<Gamma>"
+  and Empty: "P []"
+  and TyVar: "\<And>\<Gamma> a k. \<lbrakk> \<turnstile> \<Gamma> ; P \<Gamma> ; atom a \<sharp> \<Gamma> \<rbrakk> \<Longrightarrow> P (BTyVar a k # \<Gamma>)"
+  and Var: "\<And>\<Gamma> x \<tau>. \<lbrakk> \<Gamma> \<turnstile>\<^sub>t\<^sub>y \<tau> : \<star> ; atom x \<sharp> \<Gamma> \<rbrakk> \<Longrightarrow> P (BVar x \<tau> # \<Gamma>)"
+shows "P \<Gamma>"
+  using assms(1) by (induction \<Gamma> rule: Ctx_Ty_Tm.inducts(1)) (auto simp: assms)
+
+lemma Ty_induct[consumes 1, case_names Var App Unit FunArrow Forall]:
+  assumes "\<Gamma> \<turnstile>\<^sub>t\<^sub>y \<tau> : \<kappa>"
+  and Var: "\<And>\<Gamma> a k. \<lbrakk> \<turnstile> \<Gamma> ; BTyVar a k \<in> \<Gamma> \<rbrakk> \<Longrightarrow> P \<Gamma> (TyVar a) k"
+  and App: "\<And>\<Gamma> \<tau>1 \<tau>2 \<kappa>1 \<kappa>2. \<lbrakk> \<Gamma> \<turnstile>\<^sub>t\<^sub>y \<tau>1 : KArrow \<kappa>1 \<kappa>2 ; P \<Gamma> \<tau>1 (KArrow \<kappa>1 \<kappa>2) ; \<Gamma> \<turnstile>\<^sub>t\<^sub>y \<tau>2 : \<kappa>1 ; P \<Gamma> \<tau>2 \<kappa>1 \<rbrakk> \<Longrightarrow> P \<Gamma> (TyConApp \<tau>1 \<tau>2) \<kappa>2"
+  and Unit: "\<And>\<Gamma>. P \<Gamma> TyUnit \<star>"
+  and FunArrow: "\<And>\<Gamma> \<tau>1 \<tau>2. \<lbrakk> \<Gamma> \<turnstile>\<^sub>t\<^sub>y \<tau>1 : \<star> ; P \<Gamma> \<tau>1 \<star> ; \<Gamma> \<turnstile>\<^sub>t\<^sub>y \<tau>2 : \<star> ; P \<Gamma> \<tau>2 \<star> \<rbrakk> \<Longrightarrow> P \<Gamma> (\<tau>1 \<rightarrow> \<tau>2) \<star>"
+  and Forall: "\<And>\<Gamma> a k \<sigma>. \<lbrakk> BTyVar a k # \<Gamma> \<turnstile>\<^sub>t\<^sub>y \<sigma> : \<star> ; P (BTyVar a k # \<Gamma>) \<sigma> \<star> \<rbrakk> \<Longrightarrow> P \<Gamma> (\<forall> a:k. \<sigma>) \<star>"
+shows "P \<Gamma> \<tau> \<kappa>"
+  using assms(1) by (induction \<Gamma> \<tau> \<kappa> rule: Ctx_Ty_Tm.inducts(2)) (auto simp: assms)
+
+lemma Tm_induct[consumes 1, case_names Var Abs App TAbs TApp Unit Let]:
+  assumes "\<Gamma> \<turnstile> e : \<tau>"
+  and Var: "\<And>\<Gamma> x \<tau>. \<lbrakk> \<turnstile> \<Gamma> ; BVar x \<tau> \<in> \<Gamma> \<rbrakk> \<Longrightarrow> P \<Gamma> (Var x) \<tau>"
+  and Abs: "\<And>\<Gamma> x \<tau>1 e \<tau>2. \<lbrakk> BVar x \<tau>1 # \<Gamma> \<turnstile> e : \<tau>2 ; P (BVar x \<tau>1 # \<Gamma>) e \<tau>2 \<rbrakk> \<Longrightarrow> P \<Gamma> (\<lambda> x:\<tau>1. e) (\<tau>1 \<rightarrow> \<tau>2)"
+  and App: "\<And>\<Gamma> e1 e2 \<tau>1 \<tau>2. \<lbrakk> \<Gamma> \<turnstile> e1 : (\<tau>1 \<rightarrow> \<tau>2) ; P \<Gamma> e1 (\<tau>1 \<rightarrow> \<tau>2) ; \<Gamma> \<turnstile> e2 : \<tau>1 ; P \<Gamma> e2 \<tau>1 \<rbrakk> \<Longrightarrow> P \<Gamma> (App e1 e2) \<tau>2"
+  and TAbs: "\<And>\<Gamma> a k e \<sigma>. \<lbrakk> BTyVar a k # \<Gamma> \<turnstile> e : \<sigma> ; P (BTyVar a k # \<Gamma>) e \<sigma> \<rbrakk> \<Longrightarrow> P \<Gamma> (\<Lambda> a:k. e) (\<forall> a:k. \<sigma>)"
+  and TApp: "\<And>\<Gamma> a k e \<sigma> \<tau>. \<lbrakk> \<Gamma> \<turnstile> e : (\<forall> a:k. \<sigma>) ; P \<Gamma> e (\<forall> a:k. \<sigma>) ; \<Gamma> \<turnstile>\<^sub>t\<^sub>y \<tau> : k \<rbrakk> \<Longrightarrow> P \<Gamma> (TyApp e \<tau>) \<sigma>[\<tau>/a]"
+  and Unit: "\<And>\<Gamma>. P \<Gamma> Unit TyUnit"
+  and Let: "\<And>\<Gamma> e1 e2 \<tau>1 \<tau>2 x. \<lbrakk> \<Gamma> \<turnstile> e1 : \<tau>1 ; P \<Gamma> e1 \<tau>1 ; BVar x \<tau>1 # \<Gamma> \<turnstile> e2 : \<tau>2 ; P (BVar x \<tau>1 # \<Gamma>) e2 \<tau>2 \<rbrakk> \<Longrightarrow> P \<Gamma> (Let x \<tau>1 e1 e2) \<tau>2"
+shows "P \<Gamma> e \<tau>"
+  using assms(1) by (induction \<Gamma> e \<tau> rule: Ctx_Ty_Tm.inducts(3)) (auto simp: assms)
 
 end
